%----------------------------------------------------------------------------------------
%	SOLUTION 2
%----------------------------------------------------------------------------------------
\subsection*{Problem 2}
For a valid joint pdf, it needs to satisfy,
\begin{align*}
	\int_{-\infty}^{\infty}\int_{-\infty}^{\infty} f_{XY}(u,z) du dz = 1.
\end{align*}
Substituting the expression of $f_{XY}(x,y)$ and assuming $a >0$, we get,
\begin{align*}
	& \int_{0}^{\infty}\int_{0}^{\infty} a e^{-2u}e^{-3z} du dz = 1\\
	\implies & \int_{0}^{\infty} e^{-2u}\left[\int_{0}^{\infty}e^{-3z}dz\right] du = \frac{1}{a}\\
	\implies & \int_{0}^{\infty} e^{-2u}\left[-\frac{1}{3}e^{-3z}\right]_0^{\infty}du = \frac{1}{a}\\
	\implies & \frac{1}{3}\int_{0}^{\infty} e^{-2u}du = \frac{1}{a}\\
	\implies & \frac{1}{3}\left[-\frac{1}{2}e^{-2u}\right]_0^{\infty} = \frac{1}{a}\\
	\implies & \frac{1}{3}\frac{1}{2} = \frac{1}{a}\\
	\implies & a = 6.
\end{align*}
\paragraph{(b)}First let us calculate marginal pdf of $X$ which is given by,
\begin{align}\label{eq:q2_x_marginal_pdf}
	f_X(x) &= \int_{-\infty}^{\infty}f_{XY}(x,z) dz \nonumber\\
	&= 6e^{-2x}\int_{0}^{\infty}e^{-3z}dz \nonumber\\
	&= 6e^{-2x}\left[-\frac{1}{3}e^{-3z}\right]_0^{\infty} \nonumber\\
	&= 6e^{-2x}\frac{1}{3} \nonumber\\
	&= 2e^{-2x},
\end{align}
if $x >0$ and $0$ otherwise. Therefore, we can see that $X \sim exp(2)$, $i.e.$ an exponential random variable with parameter value equals to $2$. Now, to find $\bar{x}$, we can compute the expectation of $X$ as follows,
\begin{align}\label{eq:q2_x_mean}
	\mathbb{E}[X] &= \int_{-\infty}^{\infty} uf_X(u)du \nonumber\\
	&= 2\int_{0}^{\infty}ue^{-2u}du \nonumber\\
	&= \frac{1}{2}\hspace{1cm} [\text{ from }(\ref{eq:exp_expectation})].
\end{align}
Similarly, we can find the marginal pdf of $Y$ as follows:
\begin{align}\label{eq:q2_y_marginal_pdf}
	f_Y(y) &= \int_{-\infty}^{\infty}f_{XY}(u,y) du \nonumber\\
	&= 6e^{-3y}\int_{0}^{\infty}e^{-2u}du \nonumber\\
	&= 6e^{-3y}\left[-\frac{1}{2}e^{-2u}\right]_0^{\infty} \nonumber\\
	&= 6e^{-3y}\frac{1}{2} \nonumber\\
	&= 3e^{-3y},
\end{align}
if $y >0$ and $0$ otherwise. Therefore, we can see that $Y \sim exp(3)$, $i.e.$ an exponential random variable with parameter value equals to $3$. Now, to find $\bar{y}$, we can compute the expectation of $Y$ as follows,
\begin{align}\label{eq:q2_y_mean}
	\mathbb{E}[Y] &= \int_{-\infty}^{\infty} zf_Y(z)dz \nonumber\\
	&= 3\int_{0}^{\infty}ze^{-3z}dz \nonumber\\
	&= \frac{1}{3}\hspace{1cm} [\text{ from }(\ref{eq:exp_expectation})].
\end{align}
\paragraph{(c)}The second moment of $X$ is given by,
\begin{align}\label{eq:q2_x_sec_moment}
	\mathbb{E}[X^2] &= \int_{-\infty}^{\infty} u^2f_X(u) du\nonumber\\
	&= \frac{2}{2^2}\hspace{1cm} [\text{ from }(\ref{eq:exp_sec_moment})]\nonumber\\
	&= \frac{1}{2}.
\end{align}
Similarly, the second moment of $Y$ is given by,
\begin{align}\label{eq:q2_y_sec_moment}
	\mathbb{E}[Y^2] &= \int_{-\infty}^{\infty} z^2f_Y(z) dz\nonumber\\
	&= \frac{2}{3^2}\hspace{1cm} [\text{ from }(\ref{eq:exp_sec_moment})]\nonumber\\
	&= \frac{2}{9}.
\end{align}
Now, from~(\ref{eq:q2_x_marginal_pdf}) and~(\ref{eq:q2_y_marginal_pdf}), we can see that,
\begin{align}\label{eq:q2_xy_independent}
	f_{XY}(x,y) = f_X(x)f_Y(y).
\end{align}
Therefore, by definition, $X$ and $Y$ are independent. Hence,
\begin{align}\label{eq:q2_xy_mean}
	\mathbb{E}[XY] &= \mathbb{E}[X]\mathbb{E}[Y]\nonumber\\
	&= \frac{1}{2}\frac{1}{3}\nonumber\\
	&= \frac{1}{6}.
\end{align}
\paragraph{(d)}The autocorrelation matrix of the random vector $[X\ Y]^T$ is given by,
\begin{align}
	 \mathbb{E}[[X\ Y]^T [X\ Y]] &= \begin{bmatrix}\mathbb{E}[X^2]&\mathbb{E}[XY]\\\mathbb{E}[YX]&\mathbb{E}[Y^2]\end{bmatrix}\nonumber\\
	 &= \begin{bmatrix}\frac{1}{2}&\frac{1}{6}\\\frac{1}{6}&\frac{2}{9}\end{bmatrix}.
\end{align}
\paragraph{(e)}The variance of $X$ is given by,
\begin{align}
	\mathbb{E}[(X-\mathbb{E}[X])^2] &= \mathbb{E}[X^2]-(\mathbb{E}[X])^2\nonumber\\
	&= \frac{1}{2}-\frac{1}{4}\nonumber\\
	&= \frac{1}{4}.
\end{align}
The variance of $Y$ is given by,
\begin{align}
	\mathbb{E}[(Y-\mathbb{E}[Y])^2] &= \mathbb{E}[Y^2]-(\mathbb{E}[Y])^2\nonumber\\
	&= \frac{2}{9}-\frac{1}{9}\nonumber\\
	&= \frac{1}{9}.
\end{align}
The covariance of $X$ and $Y$ is given by,
\begin{align}
	C_{XY} &= \mathbb{E}[(X-\mathbb{E}[X])(Y-\mathbb{E}[Y])]\nonumber\\
	&= \mathbb{E}[XY-X\mathbb{E}[Y]-Y\mathbb{E}[X]-\mathbb{E}[X]\mathbb{E}[Y]]\nonumber\\
	&= \mathbb{E}[XY]-\mathbb{E}[X]\mathbb{E}[Y]\nonumber\\
	&= \frac{1}{6}-\frac{1}{2}\frac{1}{3}\nonumber\\
	&= 0.
\end{align}
\paragraph{(f)}The autocovariance of the random vector $[X\ Y]^T$ is given by,
\begin{align}
	\mathbb{E}[[(X-\mathbb{E}[X])\ (Y-\mathbb{E}[Y])]^T[(X-\mathbb{E}[X])\ (Y-\mathbb{E}[Y])]] &= \begin{bmatrix}\mathbb{E}[(X-\mathbb{E}[X])^2] & \mathbb{E}[(X-\mathbb{E}[X])(Y-\mathbb{E}[Y])]\nonumber\\ \mathbb{E}[(Y-\mathbb{E}[Y])(X-\mathbb{E}[]X)] & \mathbb{E}[(Y-\mathbb{E}[Y])^2]\end{bmatrix}\nonumber\\
	&= \begin{bmatrix}\frac{1}{4} & 0\\0 & \frac{1}{9}\end{bmatrix}.
\end{align}
\paragraph{(g)} The correlation coefficient between $X$ and $Y$ is
\begin{align*}
	\rho = \frac{C_{XY}}{\sigma_x \sigma_y} = 0.
\end{align*}
\paragraph{(h)} Yes, $X$ and $Y$ are independent as we have already derived in the previous sections and shown that $f_{XY}(x,y) = f_X(x)f_Y(y)$ in~(\ref{eq:q2_xy_independent}).